fairness/examples/comp/client_defs.v
@@ -1,0 +1,214 @@
+From iris.proofmode Require Import tactics.
+From trillium.program_logic Require Export weakestpre.
+From trillium.fairness Require Import fuel_ext resources.
+From trillium.fairness.heap_lang Require Import notation.
+From iris.base_logic.lib Require Import invariants.
+From iris.prelude Require Import options.
+From iris.algebra Require Import excl_auth auth gmap gset excl.
+From iris.bi Require Import bi.
+From trillium.fairness Require Import lm_fair. 
+From trillium.fairness.ext_models Require Import ext_models.
+From trillium.fairness.examples.comp Require Import lib lib_ext.
+From trillium.fairness.heap_lang Require Export lang.
+
+Close Scope Z_scope.
+
+Section ClientDefs.
+
+  Definition lib_gs: gset lib_grole := {[ ρlg ]}.
+
+  Lemma lib_gs_ne: lib_gs ≠ ∅.
+  Proof. done. Qed.
+  Lemma ρlg_in_lib_gs: ρlg ∈ lib_gs.
+  Proof. done. Qed. 
+
+  Definition lf := lib_fair _ lib_gs_ne.
+
+  Let lib_st := fmstate lf.
+  (* Let lib_role := fmrole lib_fair. *)
+  Let lib_erole := @ext_role _ (@ExtLibLM _ lib_gs_ne). 
+
+  Definition client_state: Type := lib_st * nat.
+
+  Inductive y_role := ρy.
+  Definition client_role: Type := lib_erole + y_role.
+
+  Definition ρ_cl: client_role := inr ρy.
+  Definition ρ_lib: client_role := inl $ inl ρlg.
+  Definition ρ_ext: client_role := inl $ inr $ env (eiG ρlg) (EM := (@ExtLibLM _ lib_gs_ne)). 
+  
+  Inductive client_trans: client_state -> option client_role -> client_state -> Prop :=
+  | ct_y_step_3 lb:
+    client_trans (lb, 3) (Some ρ_cl) (lb, 2)
+  (* TODO: allow arbitrary library's LM roles *)
+  | ct_lib_ext lb (STOP: lm_is_stopped ρlg lb):
+    client_trans (lb, 2) (Some ρ_ext) (reset_lm_st ρlg lb ρlg_in_lib_gs, 1)
+  | ct_lib_step lb1 lb2 (LIB_STEP: fmtrans lf lb1 (Some ρlg) lb2):
+    client_trans (lb1, 1) (Some ρ_lib) (lb2, 1)
+  | ct_y_step_1 (lb: fmstate lf)
+                (* (LIB_NOSTEP: 0 ∉ live_roles _ lb) *)
+                (LIB_NOROLES: ls_tmap lb (LM := lib_model lib_gs) !! ρlg = Some ∅)
+    :
+    client_trans (lb, 1) (Some ρ_cl) (lb, 0)
+  .
+
+  Global Instance lib_role_EqDec: EqDecision lib_erole.
+  Proof. solve_decision. Defined.
+  Global Instance lib_role_Cnt: Countable lib_erole.
+  Proof using.
+    rewrite /lib_erole. simpl. apply _.
+  Defined.
+  
+  Instance y_EqDec: EqDecision y_role.
+  Proof. by (solve_decision). Qed.
+
+  Global Instance client_role_Cnt: Countable client_role.
+  Proof using.
+    rewrite /client_role.
+    unshelve eapply sum_countable.
+    eauto. eapply (inj_countable' (fun _ => ()) (fun _ => ρy)).
+    by destruct x.
+  Qed.
+
+  (* Instance lib_step_dec (st: client_state) (ρ: client_role) st': *)
+  (*   Decision (client_trans st (Some ρ) st'). *)
+  (* Proof. *)
+  (*   Local Ltac nostep := right; intros T; inversion T. *)
+  (*   destruct st as [δ_lib n], st' as [δ'_lib n']. *)
+  (*   destruct (decide (n = S n' /\ ρ = inr ρy /\ δ_lib = δ'_lib)), *)
+  (*            (decide (n = 1 /\ n' = 1 /\ ρ = inl ρlg)). *)
+  (*   { lia. } *)
+  (*   3: { nostep; subst; tauto. } *)
+  (*   - destruct a as (->&->&<-). *)
+  (*     destruct n'; [| destruct n'].  *)
+  (*     + destruct (ls_tmap δ_lib (LM := lib_model) !! ρlg) eqn:LIB_OBLS. *)
+  (*       2: { nostep. by rewrite LIB_OBLS in LIB_NOROLES. } *)
+  (*       destruct (decide (g = ∅)). *)
+  (*       * subst. left. by constructor.  *)
+  (*       * nostep. rewrite LIB_OBLS in LIB_NOROLES. set_solver. *)
+  (*     + left. econstructor. *)
+  (*     + nostep. *)
+  (*   - destruct a as (->&->&->). *)
+  (*     destruct (decide (locale_trans δ_lib ρlg δ'_lib (LM := lib_model))).  *)
+  
+  Instance client_step_dec (st: client_state) (ρ: client_role):
+    Decision (exists st', client_trans st (Some ρ) st').
+  Proof.
+    Local Ltac nostep := right; intros [? T]; inversion T.
+    destruct st as [δ_lib n]. destruct n; [| destruct n]; [..| destruct n]; [..| destruct n]. 
+    - by nostep. 
+    - destruct ρ.
+      + destruct l.
+        2: by nostep. 
+        destruct f.
+        pose proof (@lib_LF _ lib_gs_ne). (* why it's not inferred anymore? *)
+        destruct (decide (exists δ'_lib, locale_trans δ_lib () δ'_lib (LM := lib_model lib_gs))).
+        ** left. destruct e. eexists. econstructor. simpl. eauto.
+        ** nostep. simpl in LIB_STEP. eauto. 
+      + destruct y. 
+        destruct (ls_tmap δ_lib (LM := lib_model lib_gs) !! ρlg) eqn:LIB_OBLS.
+        2: { nostep. by rewrite LIB_OBLS in LIB_NOROLES. }
+        destruct (decide (g = ∅)).
+        * subst. left. eexists. by constructor. 
+        * nostep. rewrite LIB_OBLS in LIB_NOROLES. set_solver.
+    - destruct ρ; [destruct l| ]. 
+      1, 3: by nostep. 
+      destruct e. destruct (decide (i ∈ active_exts δ_lib)).
+      + left. destruct i. 
+        apply active_exts_spec in e as [??]. simpl in *. 
+        eexists. destruct ρlg. 
+        eapply ct_lib_ext; eauto.
+        apply H.
+      + nostep. subst. apply n. apply active_exts_spec.
+        inversion T. subst. simpl.
+        eexists. red. eauto.
+        Unshelve. apply ρlg_in_lib_gs. 
+    - destruct ρ.
+      + nostep.
+      + destruct y. left. eexists. constructor.
+    - nostep. 
+  Qed.
+
+  Definition client_lr (st: client_state): gset (client_role) :=
+    filter (fun r => (@bool_decide _ (client_step_dec st r) = true))  
+      {[ ρ_lib; ρ_ext; ρ_cl ]}. 
+
+  Lemma client_lr_spec: ∀ (s : client_state) (ρ : client_role),
+      (exists s', client_trans s (Some ρ) s') <-> ρ ∈ client_lr s.
+  Proof.
+    intros ??. rewrite /client_lr.
+    rewrite elem_of_filter. rewrite @bool_decide_eq_true.
+    rewrite !elem_of_union. rewrite !elem_of_singleton. 
+    split.
+    2: tauto. 
+    intros [? TRANS]. split; eauto. inversion TRANS; subst; eauto.
+  Qed.
+
+  Definition client_model_impl: FairModel.
+  Proof.
+    refine ({|
+        fmstate := client_state; 
+        fmrole := client_role;
+        fmtrans := client_trans;
+        live_roles := client_lr;
+    |}).
+    - pose proof (@LS_eqdec _ _ _ _ (@lib_LF _ lib_gs_ne)). (* not inferred? *)
+      solve_decision.       
+    - intros. eapply client_lr_spec; eauto. 
+  Defined.
+
+  
+    (* forall k δo_k gi, lmtr_o S!! k = Some δo_k -> *)
+    (*              (exists (δi: LiveState Gi Mi LSIi) (ρi: fmrole Mi), *)
+    (*                 state_rel (ls_under δo_k) δi /\ *)
+    (*                 ls_mapping δi !! ρi = Some gi) -> *)
+    (*              lift_Gi gi ∈ dom (ls_mapping δo_k).  *)
+  Definition client_LSI (s: client_state)
+    (m: gmap (fmrole client_model_impl) (locale heap_lang))
+    (_: gmap (fmrole client_model_impl) nat) :=
+    forall gi, (exists ρi, ls_mapping s.1 !! ρi = Some gi) -> inl $ inl gi ∈ dom m.
+    
+  Definition client_fl := 15. 
+  Definition client_model: LiveModel (locale heap_lang) client_model_impl client_LSI :=
+    {| lm_fl _ := client_fl; |}.  
+
+  Class clientPreGS (Σ: gFunctors) := ClientPreGS {
+     cl_pre_y_st :> inG Σ (authUR (optionR (exclR natO)));
+     cl_lib_preΣ :> fairnessGpreS (lib_model lib_gs) Σ;
+  }.
+
+  Class clientGS Σ := ClientGS {
+    cl_pre_inG :> clientPreGS Σ;
+    cl_y_st_name : gname;
+    cl_lib_Σ :> fairnessGS (lib_model lib_gs) Σ;
+  }.
+
+End ClientDefs. 
+
+Section ClientRA.
+  Context `{EM: ExecutionModel heap_lang M} `{@heapGS Σ _ EM} {cG: clientGS Σ}.
+  Context `{PMPP: @PartialModelPredicatesPre (locale heap_lang) _ _ Σ client_model_impl}.
+  
+  Notation "'lib_inn_role'" := (fmrole lib_model_impl).
+  Notation "'lib_inn_state'" := (fmstate lib_model_impl).
+  Notation "'lib_state'" := (fmstate lib_fair).
+
+  Definition y_auth_model_is (y: nat): iProp Σ :=
+    own cl_y_st_name (● Excl' y).
+
+  Definition y_frag_model_is (y: nat): iProp Σ :=
+    own cl_y_st_name (◯ Excl' y).
+
+  Definition client_inv_impl (st: client_state) : iProp Σ :=
+    let (lb, y) := st in
+    partial_model_is st ∗
+    y_auth_model_is y ∗
+    (* lib_msi lb.  *)
+    model_state_interp lb (fG := cl_lib_Σ).
+
+  Definition Ns := nroot .@ "client".
+
+  Definition client_inv: iProp Σ :=
+    inv Ns (∃ (st: client_state), client_inv_impl st).
+
+End ClientRA.
