fairness/examples/comp/comp_lib_pmp.v
@@ -1,0 +1,724 @@
+From iris.proofmode Require Import tactics.
+From trillium.program_logic Require Export weakestpre.
+From trillium.fairness Require Import fuel_ext resources.
+From trillium.fairness.heap_lang Require Import notation.
+From iris.base_logic.lib Require Import invariants.
+From iris.prelude Require Import options.
+From iris.algebra Require Import excl_auth auth gmap gset excl.
+From iris.bi Require Import bi.
+From trillium.fairness Require Import lm_fair. 
+From trillium.fairness.ext_models Require Import ext_models.
+From trillium.fairness.examples.comp Require Import lib lib_ext client_defs.
+From trillium.fairness.heap_lang Require Export lang.
+
+Close Scope Z_scope.
+
+  (* TODO: move *)
+  Lemma set_filter_equiv:
+  ∀ {A C : Type} {H : ElemOf A C} {H0 : Empty C} {H1 : Singleton A C} 
+    {H2 : Union C} {H3 : Intersection C} {H4 : Difference C} 
+    {H5 : Elements A C} {EqDecision0 : EqDecision A}
+    {LL: LeibnizEquiv C}
+    {FS: FinSet A C}
+    (P1 P2 : A → Prop)
+    (DEC1: ∀ x : A, Decision (P1 x)) (DEC2: ∀ x : A, Decision (P2 x))
+    (P_EQ: forall x, P1 x <-> P2 x)
+    (c1 c2: C)
+    (EQUIV: c1 ≡ c2)
+    ,
+    filter P1 c1 = filter P2 c2.
+  Proof. set_solver. Qed.
+
+  (* TODO: move *)
+  Lemma set_filter_and:
+  ∀ {A C : Type} {H : ElemOf A C} {H0 : Empty C} {H1 : Singleton A C} 
+    {H2 : Union C} {H3 : Intersection C} {H4 : Difference C} 
+    {H5 : Elements A C} {EqDecision0 : EqDecision A}
+    {LL: LeibnizEquiv C}
+    {FS: FinSet A C}
+    (P1 P2 : A → Prop)
+    (DEC1: ∀ x : A, Decision (P1 x)) (DEC2: ∀ x : A, Decision (P2 x))
+    (c: C)
+    ,
+    filter P1 (filter P2 c) = filter (fun x => P1 x /\ P2 x) c.
+  Proof. set_solver. Qed. 
+
+  (* TODO: move *)
+  Lemma set_filter_comm:
+  ∀ {A C : Type} {H : ElemOf A C} {H0 : Empty C} {H1 : Singleton A C} 
+    {H2 : Union C} {H3 : Intersection C} {H4 : Difference C} 
+    {H5 : Elements A C} {EqDecision0 : EqDecision A}
+    {LL: LeibnizEquiv C}
+    {FS: FinSet A C}
+    (P1 P2 : A → Prop)
+    (DEC1: ∀ x : A, Decision (P1 x)) (DEC2: ∀ x : A, Decision (P2 x))
+    (c: C)
+    ,
+    filter P1 (filter P2 c) = filter P2 (filter P1 c). 
+  Proof. set_solver. Qed. 
+
+  (* TODO: move *)
+  Lemma filter_singleton_if:
+  ∀ {A C : Type} {H : ElemOf A C} {H0 : Empty C} {H1 : Singleton A C} 
+    {H2 : Union C} {H3 : Intersection C} {H4 : Difference C} 
+    {H5 : Elements A C} {EqDecision0 : EqDecision A},
+    FinSet A C
+    → ∀ (P : A → Prop) {H7 : ∀ x : A, Decision (P x)} (x : A),
+        filter P ({[x]} : C) ≡ if decide (P x) then {[x]} else ∅.
+  Proof. intros. destruct decide; set_solver. Qed. 
+
+
+Section LibPMP. 
+  Context `{EM: ExecutionModel heap_lang M} `{@heapGS Σ _ EM} {cpG: clientPreGS Σ}.
+  Context `{PMPP: @PartialModelPredicatesPre (locale heap_lang) _ _ Σ client_model_impl}.
+
+  Notation "'LSG' Einvs" := (LM_steps_gen Einvs (EM := EM) (iLM := client_model) (PMPP := PMPP) (eGS := heap_fairnessGS)) (at level 10).
+
+  Tactic Notation "specialize_full" ident(H) :=
+    let foo := fresh in
+    evar (foo : Prop); cut (foo); subst foo; cycle 1; [eapply H|try clear H; intro H].
+
+  Lemma live_roles_1 lb:
+    live_roles client_model_impl (lb, 1) =
+    if (decide (ρlg ∈ live_roles _ lb))
+    then {[ ρ_lib ]}
+    else if decide (ls_tmap lb (LM := lib_model lib_gs) !! ρlg = Some ∅)
+         then {[ ρ_cl ]}
+         else ∅.
+  Proof.
+    simpl. rewrite /client_lr.
+    apply leibniz_equiv. rewrite !filter_union.
+
+    erewrite filter_singleton_not with (x := ρ_ext). 
+    2: { rewrite bool_decide_eq_false_2; [done| ].
+         intros [? STEP]. inversion STEP. }
+    rewrite union_empty_r. 
+
+    destruct (decide (ρlg ∈ live_roles lf lb)) as [LR | LR].
+    - pose proof (LM_live_role_map_notempty _ _ LR) as (?&MAP&?).
+      erewrite filter_singleton, filter_singleton_not, decide_True.
+      + set_solver.
+      + eauto.
+      + rewrite bool_decide_eq_false_2; [done| ].
+        intros [? STEP]. inversion STEP. subst. set_solver.
+      + rewrite bool_decide_eq_true_2; [done| ].
+        eapply LM_live_roles_strong in LR as [? ?]. eauto.
+        eexists. eapply ct_lib_step. simpl. eauto.
+    - rewrite filter_singleton_not; [rewrite decide_False| ].
+      2: { intros [DOM LIVE]%elem_of_filter.
+           by apply LM_live_roles_strong in DOM. }
+      2: { rewrite bool_decide_eq_false_2; [done| ].
+           intros [? STEP]. inversion STEP. subst. simpl in LIB_STEP.
+           destruct LR. apply LM_live_roles_strong. eauto. }
+      destruct (ls_tmap lb (LM := lib_model lib_gs) !! ρlg) eqn:MAP0.
+      (* ; rewrite MAP0. *)
+      + destruct (decide (g = ∅)) as [-> | ?].
+        * erewrite decide_True; [| done].
+          rewrite filter_singleton; [set_solver| ].
+          rewrite bool_decide_eq_true_2; [done| ]. eexists. by econstructor.
+        * erewrite decide_False.
+          2: { intros [=]. done. }
+          rewrite filter_singleton_not; [set_solver| ].
+          rewrite bool_decide_eq_false_2; [done| ].
+          intros [? STEP]. inversion STEP. subst.
+          rewrite MAP0 in LIB_NOROLES. congruence.
+      + erewrite decide_False; [| done].
+        rewrite filter_singleton_not; [set_solver| ].
+        rewrite bool_decide_eq_false_2; [done| ].
+        intros [? STEP]. inversion STEP. subst.
+        rewrite MAP0 in LIB_NOROLES. congruence.
+  Qed.
+
+  Lemma live_roles_3 lb0:
+    live_roles client_model_impl (lb0, 3) ≡ {[ ρ_cl ]}.
+  Proof.
+    simpl. rewrite /client_lr.
+    rewrite !filter_union.
+    erewrite filter_singleton_not, filter_singleton_not, filter_singleton; [set_solver| ..].
+    - rewrite bool_decide_eq_true_2; [done| ]. eexists. econstructor.
+    - apply not_true_iff_false.
+      rewrite bool_decide_eq_false_2; [tauto| ].
+      intros [? STEP]. inversion STEP.
+    - apply not_true_iff_false.
+      rewrite bool_decide_eq_false_2; [tauto| ].
+      intros [? STEP]. inversion STEP.
+  Qed.
+
+  Lemma live_roles_0 lb:
+    live_roles client_model_impl (lb, 0) = ∅.
+  Proof.
+    simpl. rewrite /client_lr.
+    apply leibniz_equiv. rewrite !filter_union.
+    erewrite !filter_singleton_not; [set_solver| ..].
+    all: rewrite bool_decide_eq_false_2; [done| ].
+    all: intros [? STEP]; inversion STEP.
+  Qed.
+
+  Lemma live_roles_2 lb:
+    live_roles client_model_impl (lb, 2) =
+    if (decide (lm_is_stopped ρlg lb))
+    then {[ ρ_ext ]}
+    else ∅.
+  Proof.
+    simpl. rewrite /client_lr.
+    apply leibniz_equiv. rewrite !filter_union.
+    rewrite union_comm.
+    rewrite filter_singleton_not; [rewrite filter_singleton_not| ].
+    2, 3: rewrite bool_decide_eq_false_2; [done| ]; 
+    intros [? STEP]; by inversion STEP.
+    rewrite !union_empty_l.
+
+    unshelve erewrite set_filter_equiv with (P2 := fun r => r = ρ_ext /\ lm_is_stopped ρlg lb).
+    5: reflexivity. 
+    { intros. apply and_dec.
+      - (* TODO: infer automatically *)
+        destruct x, ρ_ext.
+        { destruct e, e0.
+          { destruct (decide (f = f0)); [left | right]; congruence. }
+          3: destruct (decide (e = e0)); [left | right]; congruence.
+          all: right; intros ?; congruence. }
+        3: { destruct (y_EqDec y y0); [left | right]; congruence. }
+        all: right; intros ?; congruence. 
+      - solve_decision. }
+    2: { intros. rewrite bool_decide_eq_true.
+         split.
+         - intros [? STEP]. inversion STEP. subst. split; eauto.
+         - intros [-> STOP]. exists ((reset_lm_st ρlg lb ρlg_in_lib_gs), 1).
+           by econstructor. }
+
+    rewrite -set_filter_and set_filter_comm.
+    erewrite set_filter_equiv.
+    3: { rewrite filter_singleton; reflexivity. }
+    2: { intros. apply iff_refl. }
+    rewrite filter_singleton_if. 
+    repeat destruct decide; reflexivity || tauto.
+    Unshelve. intros. solve_decision. 
+  Qed. 
+    
+  Lemma lib_tmap_dom_restricted (δ: fmstate lf):
+    dom (ls_tmap δ (LM := lib_model lib_gs)) ⊆ {[ ρlg ]}.
+  Proof.    
+    done.
+  Qed. 
+
+  Lemma update_client_state `{clientGS Σ} Einvs
+    (extr: execution_trace heap_lang) (mtr: auxiliary_trace M)
+    c2 (lb lb': fmstate lf) f
+    (LIB_STEP: locale_trans lb ρlg lb' (LM := lib_model lib_gs))
+    (PROG_STEP: locale_step (trace_last extr) (Some 0) c2)
+    (F_BOUND: f ≤ client_fl)
+    :
+    LSG Einvs ⊢
+    em_msi (trace_last extr) (trace_last mtr) (em_GS0 := heap_fairnessGS) -∗
+    partial_model_is (lb, 1) -∗
+    partial_free_roles_are {[ρ_cl]} -∗
+    has_fuels 0 {[ρ_lib := f]}
+    ={Einvs}=∗
+    ∃ (δ2 : M) (ℓ: mlabel M),
+      ⌜em_valid_evolution_step (Some 0) c2 (trace_last mtr) ℓ δ2⌝ ∗
+      em_msi c2 δ2 (em_GS0 := heap_fairnessGS) ∗
+      has_fuels 0 (if decide (ls_tmap lb' (LM := lib_model lib_gs) !! ρlg = Some ∅)
+                   then {[ρ_cl := client_fl]}
+                   else {[ρ_lib := f]}) ∗
+      partial_model_is (lb', 1) ∗
+      partial_free_roles_are
+      (if decide (ls_tmap lb' (LM := lib_model lib_gs) !! ρlg = Some ∅) then {[ρ_lib]} else {[ρ_cl]}).
+  Proof.
+    
+    iIntros "#PMP MSI ST FR FUELS".
+    Local Ltac dEq := destruct (decide (_ = _)).
+    Local Ltac dEl := destruct (decide (_ ∈ _)).
+    pose proof (LM_map_empty_notlive lb' ρlg (LF := (@lib_LF _ lib_gs_ne))).
+
+    pose proof (live_roles_1 lb) as LIVE. rewrite decide_True in LIVE.
+    2: { eapply LM_live_roles_strong. eexists. eauto. }
+    (* TODO: consider the case with rem ≠ ∅ *)
+    pose proof (live_roles_1 lb') as LIVE'.
+
+    remember (trace_last extr) as c1. destruct c1 as (σ1, tp1).
+    destruct c2 as (σ2, tp2).
+
+    iPoseProof (LM_steps_gen_nofork_sub with "PMP") as "PMP'". 
+    iPoseProof (update_step_still_alive_gen with "[$] [$] [$] [$] [$]") as "EM_STEP".
+    7: { apply PROG_STEP. }
+    7: { apply ct_lib_step. simpl. eauto. }
+    { rewrite LIVE LIVE'.
+      apply union_subseteq_l'.
+      dEq; dEl; set_solver. }
+    { rewrite dom_singleton.
+      assert ((if (decide (ls_tmap lb' (LM := lib_model lib_gs) !! ρlg = Some ∅))
+              then {[ ρ_lib ]}
+              else (∅: gset (fmrole client_model_impl))) ⊆ {[ρ_lib]}) as IN.
+      { dEq; set_solver. }
+      apply IN. }
+    { rewrite LIVE. set_solver. }
+    all: eauto.
+    { Unshelve.
+      2: exact (if decide (ls_tmap lb' (LM := lib_model lib_gs) !! ρlg = Some ∅)
+                then {[ ρ_cl := client_fl ]}
+                else {[ ρ_lib := f ]}).
+      destruct (decide (_=_)); set_solver. }
+    { repeat split; rewrite ?LIVE ?LIVE'.
+      - dEl.
+        2: { destruct decide; set_solver. }
+        intros _. rewrite decide_False.
+        { rewrite lookup_singleton. simpl. lia. }
+        tauto.
+      - destruct (decide (_ ∈ _)); [set_solver| ].
+        destruct (decide (_=_)); [set_solver| ].
+        rewrite !lookup_singleton. simpl. lia.
+      - set_solver.
+      - dEq; [| set_solver].
+        intros. assert (ρ' = ρ_cl) as -> by set_solver.
+        rewrite lookup_singleton. simpl. lia.
+      - dEq; set_solver.
+      - dEq; dEl; set_solver.
+      - dEq; dEl; set_solver. }
+    { red. intros. red.
+      (* TODO: move this simplification, as it occurs quite often *)
+      rewrite /update_mapping. rewrite map_imap_dom_eq.
+      2: { rewrite dom_gset_to_gmap. intro.
+           destruct (decide (k ∈ dom R)); [| done].
+           intros. by eapply elem_of_dom. }
+      rewrite dom_gset_to_gmap. intros g' IN'.
+      red in H2.
+      (* at this point we must ensure that no new group roles  *)
+(*          were created by a lib step *)
+
+      destruct IN' as [? IN']. simpl in IN'.
+      apply (ls_mapping_tmap_corr (LM := lib_model lib_gs)) in IN' as (?&?&?).
+      pose proof (lib_tmap_dom_restricted lb') as DOML.
+      specialize (DOML g'). specialize_full DOML.
+      { apply elem_of_dom. set_solver. }
+      apply elem_of_singleton_1 in DOML. subst g'.
+      rewrite decide_False; [set_solver| ].
+      intros EMP. set_solver. }
+      
+    rewrite LIVE LIVE'.
+    iMod "EM_STEP" as (??) "(?&?&?&?&FREE)".
+    iModIntro. do 2 iExists _. iFrame.
+    
+    iApply partial_free_roles_are_Proper; [| iFrame].
+    dEl; dEq; tauto || set_solver.
+  Qed.
+
+  (* TODO: unify with model_agree ? *)
+  Lemma y_model_agree `{clientGS Σ} y1 y2:
+    ⊢ y_auth_model_is y1 -∗ y_frag_model_is y2 -∗ ⌜y1 = y2⌝.
+  Proof.
+    iIntros "Ha Hf".
+    by iDestruct (own_valid_2 with "Ha Hf") as
+      %[Heq%Excl_included%leibniz_equiv ?]%auth_both_valid_discrete.
+  Qed.
+
+  (* TODO: unify with update_model ? *)
+  Lemma y_update_model `{clientGS Σ} y1 y2 y:
+    y_auth_model_is y1 -∗ y_frag_model_is y2 ==∗ y_auth_model_is y ∗ y_frag_model_is y.
+  Proof.
+    iIntros "H1 H2". iCombine "H1 H2" as "H".
+    iMod (own_update with "H") as "[??]" ; eauto.
+    - by apply auth_update, option_local_update, (exclusive_local_update _ (Excl y)).
+    - iModIntro. iFrame.
+  Qed.
+     
+(*   Lemma big_opM_fmap': *)
+(*   ∀ {M M' : ofe} {o : M → M → M} {o' : M' → M' → M'} *)
+(*     {Monoid0 : Monoid o} {Monoid0' : Monoid o'} {K : Type} *)
+(*     {EqDecision0 : EqDecision K} {H : Countable K} *)
+(*     (f : M → M') (m : gmap K M), *)
+(*     (([^ op map] k↦y ∈ m, f <$> ({[ k := y ]}: gmap K M)): gmap K M') = (f <$> m: gmap K M'). *)
+(* (* f <$> {[k := ]} *) *)
+
+
+  (* TODO: remove tid=0 restriction ? *)
+  Let lib_pmi `{clientGS Σ} (m: gmap (locale heap_lang) (gset (fmrole lib_model_impl))): iProp Σ:=
+    (∃ (L: gset (fmrole lib_model_impl)) (Ract Rfr: gset client_role),
+        ⌜ m = {[ 0 := L ]} ⌝ ∗
+         frag_mapping_is {[ ρlg := L ]} ∗
+         (⌜ L ≠ ∅ ⌝ ∗ ⌜ Ract = {[ ρ_lib ]} /\ Rfr = {[ ρ_cl ]} ⌝ ∗ (∃ f: nat, partial_fuel_is {[ ρ_lib := f ]} ∗ ⌜ 1 <= f <= client_fl ⌝) ∨
+          ⌜ L = ∅ ⌝ ∗ ⌜ Ract = {[ ρ_cl ]} /\ Rfr = {[ ρ_lib ]} ⌝ ∗ partial_fuel_is {[ inr ρy := client_fl ]}) ∗
+        partial_mapping_is {[ 0 := Ract ]} ∗
+        partial_free_roles_are Rfr ∗
+        y_frag_model_is 1).
+  
+  Definition lib_PMPP `{clientGS Σ}:
+    @PartialModelPredicatesPre (locale heap_lang) _ _ Σ lib_model_impl.
+   refine
+    {|
+        partial_model_is := frag_model_is;
+        partial_free_roles_are := frag_free_roles_are;
+        partial_fuel_is := frag_fuel_is;
+        partial_mapping_is := lib_pmi;
+    |}.
+  Unshelve.
+  all: try (apply _ || solve_proper).
+  (* TODO: reuse proofs from resources.v *)
+  - intros.
+    rewrite /frag_fuel_is.
+    rewrite map_fmap_union. rewrite -gmap_disj_op_union.
+    2: { by apply map_disjoint_fmap. }
+    by rewrite auth_frag_op own_op.
+  - intros. rewrite /frag_free_roles_are.
+    rewrite -gset_disj_union; auto.
+    by rewrite auth_frag_op own_op.
+  - iApply own_unit.
+  Defined.
+
+  Lemma lib_open_inv `{clientGS Σ} ζ fs (FSnz : fs ≠ ∅):
+    client_inv -∗ has_fuels ζ fs (PMPP := lib_PMPP) -∗
+    |={↑Ns, ∅}=>
+    ⌜ ζ = 0 ⌝ ∗
+    (∃ lb, partial_model_is (lb, 1) (PartialModelPredicatesPre := PMPP) ∗ model_state_interp lb) ∗
+    frag_mapping_is {[ρlg := dom fs]}  ∗ y_auth_model_is 1 ∗
+    (∃ f, partial_fuel_is {[ρ_lib := f]} ∗ ⌜ 1 <= f <= client_fl ⌝) ∗
+    partial_mapping_is {[0 := {[ρ_lib]}]} ∗
+    partial_free_roles_are {[inr ρy]} ∗ y_frag_model_is 1 ∗
+    frag_fuel_is fs ∗
+    (▷ (∃ st, client_inv_impl st) ={ ∅, ↑Ns}=∗ emp).
+  Proof.
+    iIntros "#INV FUELS_LIB".
+    iInv Ns as ((lb, y)) ">(ST & YST_AUTH & inv')" "CLOS".
+    rewrite difference_diag_L. iModIntro.
+    iDestruct (has_fuels_equiv with "FUELS_LIB") as "[MAP_LIB FUEL_LIB]".
+    simpl. iDestruct "MAP_LIB" as (???) "(%LIBM&LM&MATCH&MAP&FR&YST)".
+    assert (ζ = 0 /\ L = dom fs) as [-> ->]; [| clear LIBM].
+    { by apply map_singleton_inj in LIBM as [-> <-]. }
+    (* assert (S <$> fs ≠ ∅) by (by intros ?%fmap_empty_inv). *)
+    iDestruct "MATCH" as "[(_&[-> ->]&(%f & Ff & %BOUND)) | [% _]]".
+    2: { exfalso. apply FSnz. apply dom_empty_iff. set_solver. }
+    iPoseProof (y_model_agree with "YST_AUTH YST") as "->".
+    iPoseProof (frag_mapping_same with "[inv'] LM") as "%TMAP0".
+    { iDestruct "inv'" as (?)"(?&?&?)". iFrame. }
+    iPoseProof (frag_fuel_included with "[inv'] [FUEL_LIB]") as "%FUEL0".
+    { iDestruct "inv'" as (?)"(?&?&?&?)". iFrame. }
+    { iApply frag_fuel_is_big_sepM; [done | by iFrame]. }
+    iSplitR; [done| ].
+    iFrame. iSplitL "ST inv'".
+    - iExists lb. iFrame. 
+    - iDestruct (frag_fuel_is_big_sepM with "FUEL_LIB") as "?"; [done| ].
+      iFrame. iExists _. iFrame. done.
+  Qed.
+
+  (* TODO: move*)
+  From trillium.fairness Require Import actual_resources.
+
+  Lemma fuel_keep_step_lifting `{clientGS Σ} Einvs (DISJ_INV: Einvs ## ↑Ns):
+  LSG Einvs ∗ client_inv ⊢
+  ∀ (extr : execution_trace heap_lang) (auxtr : auxiliary_trace M)
+    (c2 : cfg heap_lang) (fs : gmap (fmrole lib_model_impl) nat)
+    (ζ : locale heap_lang) (_ : dom fs ≠ ∅) (_ : locale_step
+                                                   (trace_last extr)
+                                                   (Some ζ) c2),
+    has_fuels ζ (S <$> fs) (PMPP := lib_PMPP) -∗
+    em_msi (trace_last extr) (trace_last auxtr) (em_GS0 := heap_fairnessGS)
+    ={Einvs ∪ ↑Ns}=∗
+    ∃ (δ2 : M) (ℓ : mlabel M),
+      ⌜em_valid_state_evolution_fairness (extr :tr[ Some ζ ]: c2)
+         (auxtr :tr[ ℓ ]: δ2)⌝ ∗
+      has_fuels ζ (filter (λ '(k, _), k ∈ dom fs ∖ ∅) fs) (PMPP := lib_PMPP) ∗
+      em_msi c2 δ2 (em_GS0 := heap_fairnessGS).
+  Proof.
+    iIntros "[#PMP #COMP]". iIntros "* FUELS_LIB MSI". simpl in *.
+    
+    assert (S <$> fs ≠ ∅) as NE.
+    { intros ?%dom_empty_iff. set_solver. }
+
+    iPoseProof (lib_open_inv with "[$] FUELS_LIB") as "INV'"; [set_solver| ].
+    rewrite union_comm_L.
+    iMod (fupd_mask_frame_r _ _ Einvs with "INV'") as
+      "(-> & (%lb & ST & inv') & LM & YST_AUTH & (%f & Ff & %BOUND) & MAP & FR & YST & FUEL_LIB & CLOS)"; [set_solver| ].
+
+    
+    iMod (actual_update_no_step_enough_fuel_keep with "[LM FUEL_LIB] inv'") as (lb') "(%LIB_STEP & FUELS_LIB & MSI_LIB & %TMAP_LIB)".
+    (* 3: { apply empty_subseteq. } *)
+    { eauto. }
+    { clear. red. intros. done. }
+    { rewrite /has_fuels_S. rewrite has_fuels_equiv. iFrame.
+      iApply frag_fuel_is_big_sepM; done. }
+    
+    destruct (trace_last extr) as (σ1, tp1) eqn:LASTE. destruct c2 as (σ2, tp2).
+    rewrite LASTE.
+    rewrite difference_empty_L.
+    (* rewrite difference_empty_L in TMAP_LIB. *)
+    iAssert (has_fuels 0 {[ ρ_lib := f ]}) with "[MAP Ff]" as "FUELS".
+    { rewrite /has_fuels. rewrite dom_singleton_L big_sepS_singleton.
+      rewrite lookup_singleton. iFrame. iExists _. iFrame. done. }
+
+    rewrite -LASTE.
+    iPoseProof (update_client_state with "[$] [$] [$] [$] [$]") as "EM_STEP"; eauto.
+    { eexists. split; [apply LIB_STEP| ]. done. }
+    { lia. }
+    iMod (fupd_mask_mono with "EM_STEP") as (δ2 ℓ) "(EV & MSI & FUELS & ST & FR)"; [set_solver| ].
+    do 2 iExists _. iFrame "EV MSI".
+    rewrite gmap_filter_dom_id. 
+
+    iDestruct ("CLOS" with "[ST MSI_LIB YST_AUTH]") as "CLOS".
+    { iNext. iExists (_, _). rewrite /client_inv_impl. iFrame. }
+    iMod (fupd_mask_frame_r _ _ Einvs with "CLOS") as "_"; [set_solver| ].
+
+    iModIntro.
+    iDestruct "FUELS" as "[MAP FUEL]". iDestruct "FUELS_LIB" as "[MAP_LIB FUELS_LIB]".
+    rewrite /has_fuels. iSplitR "FUELS_LIB".
+    2: { done. }
+    simpl. 
+    rewrite /lib_pmi. do 3 iExists _. iFrame.
+    iSplitR; [done| ].
+    (* TODO: case when domain becomes empty *)
+    iLeft. iSplitR; [done| ].
+    rewrite TMAP_LIB.
+    (* rewrite lookup_insert. *)
+
+    assert (ls_tmap lb (LM := lib_model lib_gs) !! ρlg ≠ Some ∅) as TM_NE.
+    { edestruct (locale_trans_ex_role lb ρlg lb' (LM := lib_model lib_gs)) as [? STEP].
+      { eexists. split; [apply LIB_STEP| ]. done. }
+    eapply ls_mapping_tmap_corr in STEP as (?&?&?). rewrite H1. set_solver. } 
+    
+    repeat erewrite @decide_False; try done. 
+    iSplitR.
+    - iPureIntro.  set_solver.
+    - rewrite dom_singleton_L big_sepS_singleton.
+      rewrite lookup_singleton.
+      iDestruct "FUEL" as (?) "[%EQ ?]". inversion EQ. subst.
+      iExists _. iFrame. iPureIntro. lia.
+  Qed.
+
+  Lemma lib_fuel_drop_step_preserves_LSI s rem:
+    fuel_drop_preserves_LSI s rem (LSI := LSI_groups_fixed lib_gs).
+  Proof. 
+    (* done. *)
+    red. intros. red. intros ?? IN.
+    apply map_filter_lookup_Some in IN as [??].
+    eapply H0; eauto. 
+  Qed. 
+    
+
+  (* TODO: move*)
+  Lemma fuel_drop_step_lifting `{clientGS Σ} Einvs (DISJ_INV: Einvs ## ↑Ns):
+  LSG Einvs ∗ client_inv ⊢
+  ∀ (extr : execution_trace heap_lang) (auxtr : auxiliary_trace M)
+    (c2 : cfg heap_lang) s (fs : gmap (fmrole lib_model_impl) nat)
+    rem
+    (ζ : locale heap_lang) (_ : dom fs ≠ ∅)
+
+    (_: (live_roles _ s) ∩ rem = ∅)
+    (_: rem ⊆ dom fs)
+    (_ : locale_step (trace_last extr) (Some ζ) c2),
+    has_fuels ζ (S <$> fs) (PMPP := lib_PMPP) -∗
+    partial_model_is s -∗
+    em_msi (trace_last extr) (trace_last auxtr) (em_GS0 := heap_fairnessGS)
+    ={Einvs ∪ ↑Ns}=∗
+    ∃ (δ2 : M) (ℓ : mlabel M),
+      ⌜em_valid_state_evolution_fairness (extr :tr[ Some ζ ]: c2)
+         (auxtr :tr[ ℓ ]: δ2)⌝ ∗
+      has_fuels ζ (filter (λ '(k, _), k ∈ dom fs ∖ rem) fs) (PMPP := lib_PMPP) ∗
+      partial_model_is s ∗
+      em_msi c2 δ2 (em_GS0 := heap_fairnessGS).
+  Proof.
+    iIntros "[#PMP #COMP]". iIntros "* FUELS_LIB ST_LIB MSI". simpl in *.
+    
+    assert (S <$> fs ≠ ∅) as NE.
+    { intros ?%dom_empty_iff. set_solver. }
+
+    iPoseProof (lib_open_inv with "[$] FUELS_LIB") as "INV'"; [set_solver| ].
+    rewrite union_comm_L.
+    iMod (fupd_mask_frame_r _ _ Einvs with "INV'") as
+      "(-> & (%lb & ST & inv') & LM & YST_AUTH & (%f & Ff & %BOUND) & MAP & FR & YST & FUEL_LIB & CLOS)"; [set_solver| ].
+
+    iAssert (⌜ s = ls_under lb ⌝)%I as %->.
+    { rewrite /model_state_interp.
+      iDestruct "inv'" as (?)"(?&?&?&ST_LIB'&?)".
+      (* TODO: make a lemma? *)
+      by iDestruct (own_valid_2 with "ST_LIB' ST_LIB") as
+      %[Heq%Excl_included%leibniz_equiv ?]%auth_both_valid_discrete. }
+      
+      
+    iMod (actual_update_no_step_enough_fuel_drop with "[LM FUEL_LIB] ST_LIB inv'") as (lb') "(%LIB_STEP & FUELS_LIB & ST_LIB & MSI_LIB & %TMAP_LIB)".
+    (* 3: { apply empty_subseteq. } *)
+    { eauto. }
+    4: { rewrite /has_fuels_S. rewrite has_fuels_equiv. iFrame.
+         iApply frag_fuel_is_big_sepM; done. }
+    2: { eauto. }
+    { done. }
+    { apply lib_fuel_drop_step_preserves_LSI. }
+    
+    destruct (trace_last extr) as (σ1, tp1) eqn:LASTE. destruct c2 as (σ2, tp2).
+    rewrite LASTE.
+    (* rewrite difference_empty_L. *)
+    (* rewrite difference_empty_L in TMAP_LIB. *)
+    iAssert (has_fuels 0 {[ ρ_lib := f ]}) with "[MAP Ff]" as "FUELS".
+    { rewrite /has_fuels. rewrite dom_singleton_L big_sepS_singleton.
+      rewrite lookup_singleton. iFrame. iExists _. iFrame. done. }
+
+    rewrite -LASTE.
+    iPoseProof (update_client_state with "[$] [$] [$] [$] [$]") as "EM_STEP"; eauto.
+    { eexists. split; [apply LIB_STEP| ]. done. }
+    { lia. }
+    iMod (fupd_mask_mono with "EM_STEP") as (δ2 ℓ) "(EV & MSI & FUELS & ST & FR)"; [set_solver| ].
+    do 2 iExists _. iFrame "EV MSI".
+
+    iDestruct ("CLOS" with "[ST MSI_LIB YST_AUTH]") as "CLOS".
+    { iNext. iExists (_, _). rewrite /client_inv_impl. iFrame. }
+    iMod (fupd_mask_frame_r _ _ Einvs with "CLOS") as "_"; [set_solver| ].
+
+    iModIntro.
+    iDestruct "FUELS" as "[MAP FUEL]". iDestruct "FUELS_LIB" as "[MAP_LIB FUELS_LIB]".
+
+    iFrame "ST_LIB". 
+    iSplitR "FUELS_LIB".
+    2: { rewrite dom_domain_restrict; [| set_solver]. done. }
+    simpl. rewrite dom_domain_restrict; [| set_solver].
+    rewrite /lib_pmi. do 3 iExists _. iFrame.
+    iSplitR; [done| ].
+
+    rewrite TMAP_LIB. rewrite lookup_insert.
+    destruct (decide (dom fs = rem)).
+    2: { 
+
+    iLeft.
+    iSplitR.
+    { iPureIntro. intros ?. apply n. set_solver. } 
+    (* rewrite lookup_insert. *)
+    repeat erewrite @decide_False with (P := (Some (dom fs ∖ rem) = Some ∅)).
+    (* 2-3: by intros [=]. *)
+    2, 3: intros [=]; set_solver. 
+    iSplitR.
+    { iPureIntro. set_solver. }
+    rewrite dom_singleton_L big_sepS_singleton.
+    rewrite lookup_singleton.
+    iDestruct "FUEL" as (?) "[%EQ ?]". inversion EQ. subst.
+    iExists _. iFrame. iPureIntro. lia. }
+    
+    subst rem. iRight. iSplitR.
+    { iPureIntro. set_solver. }
+    rewrite difference_diag_L. repeat erewrite decide_True.
+    2, 3: done.
+    iSplitR.
+    { iPureIntro. set_solver. }
+    rewrite dom_singleton_L big_sepS_singleton.
+    rewrite lookup_singleton.
+    iDestruct "FUEL" as (?) "[%EQ ?]". inversion EQ.
+    iFrame.         
+  Qed.
+
+
+  Lemma lib_model_step_preserves_LSI:
+  ∀ (s1 : lib_model_impl) (ρ : fmrole lib_model_impl) 
+    (s2 : lib_model_impl) (fs1 fs2 : gmap (fmrole lib_model_impl) nat),
+    model_step_preserves_LSI s1 ρ s2 fs1 fs2 (LSI := LSI_groups_fixed lib_gs).
+  Proof.
+    (* done.  *)
+    (* can be proven trivially, but the proof below should work for non-trivial Gs *)
+    intros. red. intros. red. intros ??.
+    rewrite /update_mapping. rewrite map_lookup_imap. simpl.
+    rewrite lookup_gset_to_gmap.
+    rewrite option_guard_decide.
+    destruct (decide (ρ0 ∈ _ ∖ _)); simpl. 
+    2: { congruence. }
+    destruct decide.
+    { eapply H0; eauto. }
+    intros [=->]. eapply H0; eauto.
+  Qed.
+    
+  Lemma model_step_lifting `{clientGS Σ} Einvs (DISJ_INV: Einvs ## ↑Ns):
+  LSG Einvs ∗ client_inv ⊢
+  ∀ (extr : execution_trace heap_lang) (auxtr : auxiliary_trace M)
+    (tp1 tp2 : list (language.expr heap_lang)) (σ1 σ2 : language.state heap_lang)
+    (s1 s2 : lib_model_impl) (fs1 fs2 : gmap (fmrole lib_model_impl) nat)
+    (ρ : fmrole lib_model_impl) (δ1 : M) (ζ : locale heap_lang)
+    (fr1 fr_stash : gset (fmrole lib_model_impl))
+    (_ : live_roles lib_model_impl s2 ∖ live_roles lib_model_impl s1 ⊆ fr1 ∪ dom fs1 ∩ dom fs2)
+    (_ : fr_stash ⊆ dom fs1) (_ : live_roles lib_model_impl s1
+                                  ∩ (fr_stash ∖ {[ρ]}) = ∅)
+    (_ : dom fs2 ∩ fr_stash = ∅) (_ : trace_last extr = (tp1, σ1))
+    (_ : trace_last auxtr = δ1) (_ : locale_step (tp1, σ1) (Some ζ) (tp2, σ2))
+    (_ : fmtrans lib_model_impl s1 (Some ρ) s2)
+    (_ : valid_new_fuelmap fs1 fs2 s1 s2 ρ (LM := lib_model lib_gs))
+  ,
+    has_fuels ζ fs1 (PMPP := lib_PMPP) -∗
+    partial_model_is s1 (PartialModelPredicatesPre := lib_PMPP) -∗
+    em_msi (tp1, σ1) δ1 (em_GS0 := heap_fairnessGS) -∗
+    partial_free_roles_are fr1 (PartialModelPredicatesPre := lib_PMPP)
+    ={Einvs ∪ ↑Ns}=∗
+    ∃ (δ2 : M) (ℓ : mlabel M),
+      ⌜em_valid_state_evolution_fairness (extr :tr[ Some ζ ]: (tp2, σ2))
+         (auxtr :tr[ ℓ ]: δ2)⌝ ∗
+      has_fuels ζ fs2 (PMPP := lib_PMPP) ∗
+      partial_model_is s2 (PartialModelPredicatesPre := lib_PMPP) ∗
+      em_msi (tp2, σ2) δ2 (em_GS0 := heap_fairnessGS) ∗
+      partial_free_roles_are
+        (fr1 ∖ (live_roles lib_model_impl s2 ∖ (live_roles lib_model_impl s1 ∪ dom fs1 ∩ dom fs2))
+         ∪ fr_stash) (PartialModelPredicatesPre := lib_PMPP).
+  Proof.
+    iIntros "[#PMP #COMP]". iIntros "* FUELS_LIB ST_LIB MSI FR_LIB". simpl in *.
+    
+    assert (ρ ∈ dom fs1) as DOM1ρ by apply x7.
+    assert (dom fs1 ≠ ∅ /\ fs1 ≠ ∅) as [FS1nz FS1nz'].
+    { split; intros ?; set_solver. }
+    
+    iPoseProof (lib_open_inv with "[$] FUELS_LIB") as "INV'"; [done| ].
+    rewrite union_comm_L.
+    iMod (fupd_mask_frame_r _ _ Einvs with "INV'") as
+      "(-> & (%lb & ST & inv') & LM & YST_AUTH & (%f & Ff & %BOUND) & MAP & FR & YST & FUEL_LIB & CLOS)"; [set_solver| ].
+
+    iPoseProof (LM_steps_gen_nofork_sub with "PMP") as "PMP'".
+    iMod (actual_update_step_still_alive_gen with "[LM FUEL_LIB] [$] [$] [$]") as "LIFT"; eauto.
+    2: { rewrite has_fuels_equiv. iFrame. iApply frag_fuel_is_big_sepM; done. }
+    { apply lib_model_step_preserves_LSI. }
+
+    iDestruct "LIFT" as (lb') "(%LIB_STEP & FUELS_LIB & ST_LIB & MSI_LIB & FR_LIB & %TMAP_LIB)".
+    simpl. iFrame "ST_LIB".
+    
+    iAssert (has_fuels 0 {[ ρ_lib := f ]}) with "[MAP Ff]" as "FUELS".
+    { rewrite /has_fuels. rewrite dom_singleton_L big_sepS_singleton.
+      rewrite lookup_singleton. iFrame. iExists _. iFrame. done. }
+
+    rewrite -x3 -x4. rewrite -x3 in x5.
+    iPoseProof (update_client_state with "[$] [MSI] [ST] [$] [$]") as "EM_STEP"; eauto.
+    { eexists. split; [apply LIB_STEP| ]. done. }
+    { lia. }
+    iMod (fupd_mask_mono with "EM_STEP") as (δ2 ℓ) "(EV & MSI & FUELS & ST & FR)"; [set_solver| ].
+    do 2 iExists _. iFrame "EV MSI".
+
+    iDestruct ("CLOS" with "[ST MSI_LIB YST_AUTH]") as "CLOS".
+    { iNext. iExists (_, _). rewrite /client_inv_impl. iFrame. }
+    iMod (fupd_mask_frame_r _ _ Einvs with "CLOS") as "_"; [set_solver| ].
+    iModIntro.
+
+    rewrite !has_fuels_equiv. simpl.
+    iDestruct "FUELS" as "[MAP FUELS]".
+    iDestruct "FUELS_LIB" as "[MAP' FUELS_LIB]". iFrame "FUELS_LIB FR_LIB".
+    rewrite /lib_pmi. do 3 iExists _. iFrame.
+    iSplitR; [done |].
+    rewrite TMAP_LIB. rewrite lookup_insert.
+    dEq.
+    - iRight. rewrite big_sepM_singleton. iFrame.
+      iPureIntro. set_solver.
+    - iLeft. rewrite big_sepM_singleton.
+      iApply bi.sep_assoc. iSplitR "FUELS".
+      2: { iExists _. iFrame. iPureIntro. lia. }
+      iPureIntro. split; [| set_solver]. intros ?. rewrite H1 in n. done.
+  Qed.
+
+
+  Lemma lib_PMP `{clientGS Σ} Einvs (DISJ_INV: Einvs ## ↑Ns):
+    LSG Einvs ∗ client_inv ⊢
+    (* PartialModelPredicates (Einvs ∪ ↑Ns) (LM := LM) (iLM := spinlock_model) (PMPP := (sl1_PMPP γ)).  *)
+    LM_steps_gen_nofork (Einvs ∪ ↑Ns) (EM := EM) (iLM := lib_model lib_gs) (PMPP := lib_PMPP) (eGS := heap_fairnessGS).
+  Proof.
+    iIntros "[#PMP #COMP]". iApply @Build_LM_steps_gen_nofork.
+
+    iModIntro. repeat iSplitR.
+    - iIntros "* FUELS_LIB ST MSI".
+      iDestruct (fuel_drop_step_lifting with "[$] [] [] [] [] FUELS_LIB ST MSI") as "LIFT"; eauto.
+      (* change the PMP interface so it allows fupd in fuel step *)
+      admit.      
+    - iIntros "* FUELS_LIB MSI".
+      iDestruct (fuel_keep_step_lifting with "[$] [] [] FUELS_LIB MSI") as "LIFT"; eauto.
+      (* same as above *)
+      admit.
+    - iIntros "* FUELS_LIB ST MSI FR".
+      iApply (model_step_lifting with "[$] [] [] [] [] [] [] [] [] [] [$] [$] [$] [$]"); eauto.
+  Admitted.
+
+
+End LibPMP. 
