fairness/examples/comp/traces_equiv.v
@@ -1,0 +1,132 @@
+From trillium.fairness Require Import inftraces trace_len subtrace my_omega lemmas.
+
+Local Ltac gd t := generalize dependent t.
+
+Definition traces_equiv {St L: Type} :=
+  @traces_match L L St St eq eq (fun _ _ _ => True) (fun _ _ _ => True).
+
+(* Lemma after_equiv {St L: Type} (tr1 tr *)
+(* Lemma subtrace _inf_after_equiva *)
+Lemma trace_prefix_inf_equiv_id {St L: Type} (tr: trace St L) ml len
+  (LEN: trace_len_is tr len)
+  (LE: NOmega.le len ml):
+  traces_equiv tr (trace_prefix_inf tr ml).
+Proof.
+  gd tr. gd ml. gd len. 
+  cofix CIH.
+  intros. 
+  rewrite trace_prefix_inf_step_equiv.
+  rewrite (trace_unfold_fold tr).
+  destruct tr.
+  { rewrite /trace_prefix_inf_step_alt. simpl.
+    destruct decide; by econstructor. }
+  rewrite /trace_prefix_inf_step_alt. simpl.
+  eapply trace_len_tail in LEN.
+  rewrite decide_False.
+  2: { lia_NO' ml; lia_NO' len.
+       destruct (decide (2 <= n0)).
+       { lia. }
+       replace (Nat.pred n0) with 0 in LEN; [| lia].
+       by eapply trace_len_0_inv in LEN. }
+  econstructor; try done.
+  specialize_full CIH; [| by apply LEN| by apply CIH]. 
+  lia_NO' ml; lia_NO' len. 
+Qed.
+
+
+Lemma subtrace_equiv_after {St L: Type} (tr str: trace St L) i ml len
+  (LEN: trace_len_is tr len)
+  (LE: NOmega.le len ml)
+  (SUB: subtrace tr i ml = Some str)
+  (* (DOM: NOmega.lt_nat_l start fin *)
+  :
+  exists atr, after i tr = Some atr /\
+  traces_equiv atr str.
+Proof.
+  rewrite /subtrace in SUB.
+  destruct after eqn:AFTER; [| done]. destruct decide; [done| ].
+  eexists. split; eauto.  
+  inversion SUB. subst str.
+  eapply trace_prefix_inf_equiv_id. 
+  - eapply trace_len_after; eauto.
+  - lia_NO' ml; lia_NO' len.
+Qed.
+
+
+Instance traces_equiv_refl {St L: Type}:
+  Reflexive (@traces_equiv St L). 
+Proof.
+  red. cofix CIH.
+  intros tr. rewrite (trace_unfold_fold tr).  
+  destruct tr.
+  - constructor. done. Guarded.  
+  - constructor; try done.
+    by apply CIH. 
+Qed. 
+
+
+Global Instance traces_equiv_symm {St L: Type}:
+  Symmetric (@traces_equiv St L). 
+Proof.
+  red. 
+  cofix CIH.
+  intros tr1 tr2 EQ. 
+  rewrite (trace_unfold_fold tr1) (trace_unfold_fold tr2).
+  destruct tr1, tr2.
+  - constructor. inversion EQ. done. 
+  - by inversion EQ. 
+  - by inversion EQ. 
+  - inversion EQ. subst.
+    constructor; try done.
+    by apply CIH. 
+Qed. 
+
+
+From Paco Require Import paco1 paco2 pacotac.
+Lemma upto_stutter_Proper_impl {St S' L L': Type} {Us: St -> S'} {Usls: St -> L -> St -> option L'}:
+  Proper (@traces_equiv St L ==> @traces_equiv S' L' ==> impl)
+    (upto_stutter Us Usls).
+Proof. 
+  red. intros t1 t1' EQ1 t2 t2' EQ2 UPTO.
+  gd t1. gd t2. gd t1'. gd t2'.
+  (* pcofix CIH.  *)
+  pcofix CIH. 
+  pfold.
+
+  intros. 
+  erewrite (trace_unfold_fold t1'), (trace_unfold_fold t2') in *. 
+  erewrite (trace_unfold_fold t1), (trace_unfold_fold t2) in *. 
+  (* pfold. punfold UPTO; [| admit]. *) 
+  punfold UPTO; [| apply upto_stutter_mono].
+  inversion UPTO; subst.
+  - destruct t1, t2; try done.
+    inversion EQ1; inversion EQ2; subst; try done.    
+    inversion H0. inversion H. subst.
+    destruct t1', t2'; try done.
+    inversion H2. inversion H5. subst.
+    econstructor.
+  - destruct t1, t2, t1', t2'; try by done.
+    all: inversion EQ1; inversion EQ2; subst; try by done.
+    + inversion H. simpl in H2. subst.
+      Guarded. 
+      specialize (CIH ⟨ Us s2 ⟩ t1' ⟨ Us s2 ⟩).
+      specialize CIH with (t1 := t1).
+      Guarded.
+      specialize_full CIH.
+      4: { rewrite /upaco2.
+           (* eapply upto_stutter_stutter. *)
+           (* 4: { eapply upto_stutter_stutter.  *)
+           (* 2: { econstructor.  *)
+           (* (* 2: { ??? *) *)
+           (* all: admit. } *)
+Admitted. 
+
+Instance upto_stutter_Proper {St S' L L': Type} {Us: St -> S'} {Usls: St -> L -> St -> option L'}:
+  Proper (@traces_equiv St L ==> @traces_equiv S' L' ==> iff)
+    (upto_stutter Us Usls).
+Proof. 
+  red. intros ??????. split.
+  - intros. eapply upto_stutter_Proper_impl; eauto.
+  - intros. apply traces_equiv_symm in H, H0. 
+    eapply upto_stutter_Proper_impl; eauto.
+Qed.
